src/StackCompCombined.v
@@ -15,19 +15,289 @@ Require
     StackFlatterComp2
 .
 
+Definition compile_cont (cu : ValueFlag.prog_type) : res StackCont.prog_type :=
+  OK cu
+  @@@ StackMachComp.compile_cu
+  @@ StackContComp.compile_cu.
+
+Section FSIMcont.
+
+  Variable a : ValueFlag.prog_type.
+  Variable b : StackCont.prog_type.
+  Hypothesis TRANSF : compile_cont a = OK b.
+
+  Lemma compile_cont_succ :
+    { c | StackMachComp.compile_cu a = Some c }.
+  Proof.
+    unfold compile_cont in TRANSF. break_result_chain. eauto.
+  Qed.
+  
+  Definition fsim_cont : Semantics.forward_simulation (ValueFlag.semantics a) (StackCont.semantics b).
+    destruct compile_cont_succ.
+    eapply Semantics.compose_forward_simulation;
+      try eapply StackMachComp.fsim; eauto;
+      try eapply StackContComp.fsim; eauto.
+    unfold compile_cont in *; break_result_chain.
+    congruence.
+  Defined.
+
+  Lemma fsim_cont_match_val :
+    forall x y,
+      Semantics.fsim_match_val _ _ fsim_cont x y <-> eq x y.
+  Proof.
+    intros. unfold fsim_cont.
+    destruct compile_cont_succ.
+    erewrite Semantics.fsim_match_val_compose. repeat instantiate (1 := eq).
+    split; intros; repeat break_exists; repeat eexists; repeat break_and; eauto; try congruence.
+    erewrite StackMachComp.match_val_eq.
+    intros; split; intros; congruence.
+    erewrite StackContComp.match_val_eq.
+    intros; split; intros; congruence.
+  Qed.    
+
+End FSIMcont.
+
+Definition compile_cont2 (cu : ValueFlag.prog_type) : res StackCont2.prog_type :=
+  OK cu
+  @@@ compile_cont
+  @@ StackContComp2.compile_cu.
+
+Section FSIMcont2.
+
+  Variable a : ValueFlag.prog_type.
+  Variable b : StackCont2.prog_type.
+  Hypothesis TRANSF : compile_cont2 a = OK b.
+
+  Lemma compile_cont2_succ :
+    { c | compile_cont a = Some c }.
+  Proof.
+    unfold compile_cont2 in TRANSF. break_result_chain. eauto.
+  Qed.
+  
+  Definition fsim_cont2 : Semantics.forward_simulation (ValueFlag.semantics a) (StackCont2.semantics b).
+    destruct compile_cont2_succ.
+    eapply Semantics.compose_forward_simulation;
+      try eapply fsim_cont; eauto;
+      try eapply StackContComp2.fsim; eauto.
+    unfold compile_cont2 in *; break_result_chain.
+    unfold option_to_res in *. congruence.
+  Defined.
+
+  Lemma fsim_cont2_match_val :
+    forall x y,
+      Semantics.fsim_match_val _ _ fsim_cont2 x y <-> eq x y.
+  Proof.
+    intros. unfold fsim_cont2.
+    destruct compile_cont2_succ.
+    erewrite Semantics.fsim_match_val_compose. repeat instantiate (1 := eq).
+    split; intros; repeat break_exists; repeat eexists; repeat break_and; eauto; try congruence.
+    intros. erewrite fsim_cont_match_val.
+    intros; split; intros; congruence.
+    erewrite StackContComp2.match_val_eq.
+    intros; split; intros; congruence.
+  Qed.    
+
+End FSIMcont2.
+
+Definition compile_cont3 (cu : ValueFlag.prog_type) : res StackCont3.prog_type :=
+  OK cu
+  @@@ compile_cont2
+  @@ StackContComp3.compile_cu.
+
+Section FSIMcont3.
+
+  Variable a : ValueFlag.prog_type.
+  Variable b : StackCont3.prog_type.
+  Hypothesis TRANSF : compile_cont3 a = OK b.
+
+  Lemma compile_cont3_succ :
+    { c | compile_cont2 a = Some c }.
+  Proof.
+    unfold compile_cont3 in TRANSF. break_result_chain. eauto.
+  Qed.
+  
+  Definition fsim_cont3 : Semantics.forward_simulation (ValueFlag.semantics a) (StackCont3.semantics b).
+    destruct compile_cont3_succ.
+    eapply Semantics.compose_forward_simulation;
+      try eapply fsim_cont2; eauto;
+        try eapply StackContComp3.fsim; eauto.
+    unfold compile_cont3 in *; break_result_chain.
+    unfold option_to_res in *. congruence.
+  Defined.
+
+  Lemma fsim_cont3_match_val :
+    forall x y,
+      Semantics.fsim_match_val _ _ fsim_cont3 x y <-> eq x y.
+  Proof.
+    intros. unfold fsim_cont3.
+    destruct compile_cont3_succ.
+    erewrite Semantics.fsim_match_val_compose. repeat instantiate (1 := eq).
+    split; intros; repeat break_exists; repeat eexists; repeat break_and; eauto; try congruence.
+    intros. erewrite fsim_cont2_match_val.
+    intros; split; intros; congruence.
+    erewrite StackContComp3.match_val_eq.
+    intros; split; intros; congruence.
+  Qed.    
+
+End FSIMcont3.
+
+Definition compile_flat (cu : ValueFlag.prog_type) : res StackFlat.prog_type :=
+  OK cu
+  @@@ compile_cont3
+  @@ StackFlatComp.compile_cu.
+
+Section FSIMflat.
+
+  Variable a : ValueFlag.prog_type.
+  Variable b : StackFlat.prog_type.
+  Hypothesis TRANSF : compile_flat a = OK b.
+
+  Lemma compile_flat_succ :
+    { c | compile_cont3 a = OK c }.
+  Proof.
+    unfold compile_flat in TRANSF. break_result_chain. eauto.
+  Qed.
+  
+  Definition fsim_flat : Semantics.forward_simulation (ValueFlag.semantics a) (StackFlat.semantics b).
+    destruct compile_flat_succ.
+    eapply Semantics.compose_forward_simulation;
+      try eapply fsim_cont3; eauto;
+        try eapply StackFlatComp.fsim; eauto.
+    unfold compile_flat in *; break_result_chain.
+    unfold option_to_res in *. congruence.
+  Defined.
+
+  Lemma fsim_flat_match_val :
+    forall x y,
+      Semantics.fsim_match_val _ _ fsim_flat x y <-> eq x y.
+  Proof.
+    intros. unfold fsim_flat.
+    destruct compile_flat_succ.
+    erewrite Semantics.fsim_match_val_compose. repeat instantiate (1 := eq).
+    split; intros; repeat break_exists; repeat eexists; repeat break_and; eauto; try congruence.
+    intros. erewrite fsim_cont3_match_val.
+    intros; split; intros; congruence.
+    erewrite StackFlatComp.match_val_eq.
+    intros; split; intros; congruence.
+  Qed.    
+
+End FSIMflat.
+
+Definition compile_flatter (cu : ValueFlag.prog_type) : res StackFlatter.prog_type :=
+  OK cu
+  @@@ compile_flat
+  @@ StackFlatterComp.compile_cu.
+
+Section FSIMflatter.
+
+  Variable a : ValueFlag.prog_type.
+  Variable b : StackFlatter.prog_type.
+  Hypothesis TRANSF : compile_flatter a = OK b.
+
+  Lemma compile_flatter_succ :
+    { c | compile_flat a = OK c }.
+  Proof.
+    unfold compile_flatter in TRANSF. break_result_chain. eauto.
+  Qed.
+  
+  Definition fsim_flatter : Semantics.forward_simulation (ValueFlag.semantics a) (StackFlatter.semantics b).
+    destruct compile_flatter_succ.
+    eapply Semantics.compose_forward_simulation;
+      try eapply fsim_flat; eauto;
+        try eapply StackFlatterComp.fsim; eauto.
+    unfold compile_flatter in *; break_result_chain.
+    unfold option_to_res in *. congruence.
+  Defined.
+
+  Lemma fsim_flatter_match_val :
+    forall x y,
+      Semantics.fsim_match_val _ _ fsim_flatter x y <-> eq x y.
+  Proof.
+    intros. unfold fsim_flatter.
+    destruct compile_flatter_succ.
+    erewrite Semantics.fsim_match_val_compose. repeat instantiate (1 := eq).
+    split; intros; repeat break_exists; repeat eexists; repeat break_and; eauto; try congruence.
+    intros. erewrite fsim_flat_match_val.
+    intros; split; intros; congruence.
+    erewrite StackFlatterComp.match_val_eq.
+    intros; split; intros; congruence.
+  Qed.    
+
+End FSIMflatter.
+
+Definition compile_flatter2 (cu : ValueFlag.prog_type) : res StackFlatter2.prog_type :=
+  OK cu
+  @@@ compile_flatter
+  @@ StackFlatterComp2.compile_cu.
+
+Section FSIMflatter2.
+
+  Variable a : ValueFlag.prog_type.
+  Variable b : StackFlatter2.prog_type.
+  Hypothesis TRANSF : compile_flatter2 a = OK b.
+
+  Lemma compile_flatter2_succ :
+    { c | compile_flatter a = OK c }.
+  Proof.
+    unfold compile_flatter2 in TRANSF. break_result_chain. eauto.
+  Qed.
+  
+  Definition fsim_flatter2 : Semantics.forward_simulation (ValueFlag.semantics a) (StackFlatter2.semantics b).
+    destruct compile_flatter2_succ.
+    eapply Semantics.compose_forward_simulation;
+      try eapply fsim_flatter; eauto;
+        try eapply StackFlatterComp2.fsim; eauto.
+    unfold compile_flatter2 in *; break_result_chain.
+    unfold option_to_res in *. congruence.
+  Defined.
+
+  Lemma fsim_flatter2_match_val :
+    forall x y,
+      Semantics.fsim_match_val _ _ fsim_flatter2 x y <-> eq x y.
+  Proof.
+    intros. unfold fsim_flatter2.
+    destruct compile_flatter2_succ.
+    erewrite Semantics.fsim_match_val_compose. repeat instantiate (1 := eq).
+    split; intros; repeat break_exists; repeat eexists; repeat break_and; eauto; try congruence.
+    intros. erewrite fsim_flatter_match_val.
+    intros; split; intros; congruence.
+    erewrite StackFlatterComp2.match_val_eq.
+    intros; split; intros; congruence.
+  Qed.    
+
+End FSIMflatter2.
+
+
+
+
+
 Module A := ValueFlag.
 Module B := StackFlatter2.
 
 Definition compile_cu (cu : A.env * list metadata) : res (B.env * list metadata) :=
-  OK cu
- @@@ StackMachComp.compile_cu
-  @@ StackContComp.compile_cu
-  @@ StackContComp2.compile_cu
-  @@ StackContComp3.compile_cu
-  @@ StackFlatComp.compile_cu
-  @@ StackFlatterComp.compile_cu
-  @@ StackFlatterComp2.compile_cu
-.
+  compile_flatter2 cu.
+
+Section Preservation.
+
+  Variable prog : A.prog_type.
+  Variable tprog : B.prog_type.
+
+  Hypothesis TRANSF : compile_cu prog = OK tprog.
+
+  Definition fsim : Semantics.forward_simulation (A.semantics prog) (B.semantics tprog).
+    eapply fsim_flatter2. assumption.
+  Defined.
+
+  Lemma match_val_eq :
+    forall x y,
+      Semantics.fsim_match_val _ _ fsim x y <-> eq x y.
+  Proof.
+    eapply fsim_flatter2_match_val.
+  Qed.
+
+End Preservation.
+
+
 
 Inductive I : A.state -> B.state -> Prop :=
 | ICombined : forall s00 s01 s02 s03 s04 s05 s06 s07,
@@ -74,6 +344,12 @@ Theorem compile_I_func : forall a ameta b bmeta,
     Forall2 I_func a b.
 intros0 Hcomp. unfold compile_cu in *.
 
+unfold compile_flatter2 in *.
+unfold compile_flatter in *.
+unfold compile_flat in *.
+unfold compile_cont3 in *.
+unfold compile_cont2 in *.
+unfold compile_cont in *.
 remember (a, ameta) as aprog.
 break_result_chain.
 subst aprog.  repeat on (_ * _)%type, fun x => destruct x.
@@ -91,40 +367,4 @@ Qed.
 
 
 
-Require Semantics.
 
-Section Preservation.
-
-  Variable prog : A.prog_type.
-  Variable tprog : B.prog_type.
-
-  Hypothesis TRANSF : compile_cu prog = OK tprog.
-
-  Theorem fsim :
-    Semantics.forward_simulation (A.semantics prog) (B.semantics tprog).
-  Proof.
-    unfold compile_cu in TRANSF.
-    break_result_chain.
-
-    eapply Semantics.compose_forward_simulation.
-    eapply StackMachComp.fsim; try eassumption.
-
-    eapply Semantics.compose_forward_simulation.
-    eapply StackContComp.fsim; try eassumption.
-
-    eapply Semantics.compose_forward_simulation.
-    eapply StackContComp2.fsim; try eassumption.
-
-    eapply Semantics.compose_forward_simulation.
-    eapply StackContComp3.fsim; try eassumption.
-
-    eapply Semantics.compose_forward_simulation.
-    eapply StackFlatComp.fsim; try eassumption.
-
-    eapply Semantics.compose_forward_simulation.
-    eapply StackFlatterComp.fsim; try eassumption.
-
-    eapply StackFlatterComp2.fsim; try eassumption.
-  Qed.
-
-End Preservation.
